adding many annotations to the test files to get them to compile again (not exactly sure how they were compiling before)

src/tls/test/TestDH.fst
@@ -5,7 +5,7 @@ open CoreCrypto
 open CommonDH
 open TLSConstants
 
-let main () =
+let main () : ML unit =
   let group = default_group in
   let gx = keygen group in
   let gy, gxy = dh_responder gx in
